proofs/isabelle/SpecRest/core/TranslateFullDef.thy
@@ -1,0 +1,8 @@
+theory TranslateFullDef
+  imports Translate IR_Lower
+begin
+
+definition translate_full :: "String.literal list \<Rightarrow> expr_full \<Rightarrow> smt_term option" where
+  "translate_full enums e \<equiv> map_option translate (lower enums e)"
+
+end
